src/Consensus.Tests/ContractMessageTests.fs
@@ -46,9 +46,9 @@ let setup = fun () ->
     module ET = Zen.ErrorT
     module Tx = Zen.TxSkeleton
 
-    val main: txSkeleton -> hash -> string -> data -> option lock -> #l:nat -> wallet l 
+    val main: txSkeleton -> hash -> string -> data -> option lock -> wallet
         -> result (txSkeleton ** option message) `cost` (64 + (64 + 64 + 0) + 21)
-    let main txSkeleton contractHash command data returnAddress #l wallet =
+    let main txSkeleton contractHash command data returnAddress wallet =
         if command = "contract2_test" then
         begin
             let! contractToken = Zen.Asset.getDefault contractHash in
@@ -60,8 +60,8 @@ let setup = fun () ->
         else
             ET.autoFailw "unsupported command"
     
-    val cf: txSkeleton -> string -> data -> option lock -> #l:nat -> wallet l -> cost nat 9
-        let cf _ _ _ _ #l _ = ret (64 + (64 + 64 + 0) + 21)
+    val cf: txSkeleton -> string -> data -> option lock -> wallet -> cost nat 9
+        let cf _ _ _ _ _ = ret (64 + (64 + 64 + 0) + 21)
     """
     let contract2Hash = Contract.computeHash contract2Code
 
@@ -79,9 +79,9 @@ let setup = fun () ->
             module ET = Zen.ErrorT
             module Tx = Zen.TxSkeleton
 
-            val main: txSkeleton -> hash -> string -> data -> option lock -> #l:nat -> wallet l 
+            val main: txSkeleton -> hash -> string -> data -> option lock -> wallet
                 -> result (txSkeleton ** option message) `cost` (64 + (64 + 64 + 0) + 26)
-            let main txSkeleton contractHash command data returnAddress #l wallet =
+            let main txSkeleton contractHash command data returnAddress wallet =
                 if command = "contract1_test" then
                 begin
                     let! asset = Zen.Asset.getDefault contractHash in
@@ -98,8 +98,8 @@ let setup = fun () ->
                 else
                     ET.autoFailw "unsupported command"
         
-            val cf: txSkeleton -> string -> data -> option lock -> #l:nat -> wallet l -> cost nat 9
-            let cf _ _ _ _ #l _ = ret (64 + (64 + 64 + 0) + 26)
+            val cf: txSkeleton -> string -> data -> option lock -> wallet -> cost nat 9
+            let cf _ _ _ _ _ = ret (64 + (64 + 64 + 0) + 26)
         """
 
     contracts <- result {
