src/Consensus.Tests/ContractTests.fs
@@ -99,9 +99,9 @@ let ``Contract should not be able to create tokens other than its own``() =
          module ET = Zen.ErrorT
          module Tx = Zen.TxSkeleton
 
-         val main: txSkeleton -> hash -> string -> data -> option lock -> #l:nat -> wallet l 
+         val main: txSkeleton -> hash -> string -> data -> option lock -> wallet
             -> result (txSkeleton ** option message) `cost` (64 + (64 + 64 + 0) + 21)
-         let main txSkeleton contractHash command data returnAddress #l wallet =
+         let main txSkeleton contractHash command data returnAddress wallet =
            let! asset = Zen.Asset.getDefault Zen.Asset.zeroHash in
            let lock = ContractLock contractHash in
            let spend = {
@@ -117,8 +117,8 @@ let ``Contract should not be able to create tokens other than its own``() =
 
            ET.ret (txSkeleton, None)
            
-           val cf: txSkeleton -> string -> data -> option lock -> #l:nat -> wallet l -> cost nat 9
-                    let cf _ _ _ _ #l _ = ret (64 + (64 + 64 + 0) + 21)
+           val cf: txSkeleton -> string -> data -> option lock -> wallet -> cost nat 9
+                    let cf _ _ _ _ _ = ret (64 + (64 + 64 + 0) + 21)
            """
     , (Error "illegal creation of tokens" : Result<Transaction, string>))
     |> shouldEqual
@@ -134,15 +134,15 @@ let ``Contract should be able to destroy its own tokens locked to it``() =
     module ET = Zen.ErrorT
     module Tx = Zen.TxSkeleton
 
-    val main: txSkeleton -> hash -> string -> data -> option lock -> #l:nat -> wallet l 
+    val main: txSkeleton -> hash -> string -> data -> option lock -> wallet
         -> result (txSkeleton ** option message) `cost` (64 + (64 + 0) + 11)
-    let main txSkeleton contractHash command data returnAddress #l wallet =
+    let main txSkeleton contractHash command data returnAddress wallet =
         let! asset = Zen.Asset.getDefault contractHash in
         let! txSkeleton1 = Tx.destroy 1000UL asset txSkeleton in
         ET.ret (txSkeleton1, None)
     
-    val cf: txSkeleton -> string -> data -> option lock -> #l:nat -> wallet l -> cost nat 7
-        let cf _ _ _ _ #l _ = ret (64 + (64 + 0) + 11)
+    val cf: txSkeleton -> string -> data -> option lock -> wallet -> cost nat 7
+        let cf _ _ _ _ _ = ret (64 + (64 + 0) + 11)
     
     """
 
@@ -208,14 +208,14 @@ let ``Contract should not be able to destroy tokens other than its own - single 
     module ET = Zen.ErrorT
     module Tx = Zen.TxSkeleton
 
-    val main: txSkeleton -> hash -> string -> data -> option lock -> #l:nat -> wallet l 
+    val main: txSkeleton -> hash -> string -> data -> option lock -> wallet
         -> result (txSkeleton ** option message) `cost` (64 + 8)
-    let main txSkeleton contractHash command data returnAddress #l wallet =
+    let main txSkeleton contractHash command data returnAddress wallet =
         let! txSkeleton1 = Tx.destroy 1000UL zenAsset txSkeleton in // should be impossible
         ET.ret (txSkeleton1, None)
     
-    val cf: txSkeleton -> string -> data -> option lock -> #l:nat -> wallet l -> cost nat 3
-        let cf _ _ _ _ #l _ = ret (64 + 8)
+    val cf: txSkeleton -> string -> data -> option lock -> wallet -> cost nat 3
+        let cf _ _ _ _ _ = ret (64 + 8)
     """
 
     let contractHash =
@@ -259,16 +259,16 @@ let ``Contract should not be able to destroy tokens other than its own - multipl
     module ET = Zen.ErrorT
     module Tx = Zen.TxSkeleton
 
-    val main: txSkeleton -> hash -> string -> data -> option lock -> #l:nat -> wallet l 
+    val main: txSkeleton -> hash -> string -> data -> option lock -> wallet
         -> result (txSkeleton ** option message) `cost` (64 + (64 + 64 + 0) + 15)
-    let main txSkeleton contractHash command data returnAddress #l wallet =
+    let main txSkeleton contractHash command data returnAddress wallet =
         let! asset = Zen.Asset.getDefault contractHash in
         let txSkeleton1 = Tx.destroy 1000UL zenAsset txSkeleton in // should be impossible
         let! txSkeleton2 = txSkeleton1 >>= Tx.destroy 1000UL asset in // should be possible
         ET.ret (txSkeleton2, None)
     
-    val cf: txSkeleton -> string -> data -> option lock -> #l:nat -> wallet l -> cost nat 9
-        let cf _ _ _ _ #l _ = ret (64 + (64 + 64 + 0) + 15)
+    val cf: txSkeleton -> string -> data -> option lock -> wallet -> cost nat 9
+        let cf _ _ _ _ _ = ret (64 + (64 + 64 + 0) + 15)
     """
 
     let contractHash =
