src/Zulib/fstar/Zen.Types.Extracted.fst
@@ -51,4 +51,4 @@ unopteq type blockHeader = {
     difficulty: U32.t;
     nonce: nonce }
 
-type wallet (n:nat) = pointedOutput `V.t` n
+type wallet = list pointedOutput
